@prefix cpm: <http://purl.org/voc/cpm#>.
@prefix om: <http://def.seegrid.csiro.au/isotc211/iso19156/2011/observation#>.
@prefix proc: <http://www.example.org/ont/complex-processes>.
@prefix prov: <http://www.w3.org/ns/prov#>.
@prefix rdf: <http://www.w3.org/1999/02/22-rdf-syntax-ns#>.
@prefix rdfs: <http://www.w3.org/2000/01/rdf-schema#>.
@prefix sam: <http://def.seegrid.csiro.au/isotc211/iso19156/2011/sampling#>.
@prefix skos: <http://www.w3.org/2004/02/skos/core#>.
@prefix vann: <http://purl.org/vocab/vann/>.

proc:ComplexProcess a rdfs:Class;
	rdfs:label "ComplexProcess"@en;
	rdfs:comment "The ComplexProcess class "@en;
	rdfs:subClassOf sam:Process;
	rdfs:subClassOf om:Process;
	rdfs:subClassOf prov:Activity. 

proc:Instrument a rdfs:Class;
	rdfs:subClassOf prov:Agent;
	rdfs:label "The Instrument class describes characteristics of the sensor used to generate an Observation"@en.

proc:Quality a rdfs:Class;
	rdfs:label "The Quality class retains information about the Process such as Limits of Detection; Uncertainity; Accuracy and Precision"@en.

proc:Algorithm a rdfs:Class;
	rdfs:subClassOf prov:Entity;
	rdfs:label "Algorithm"@en;
	rdfs:comment "The Algorithm class is used to describe data processing equations and calculations."@en.

proc:ManufacturersCalibration a rdfs:Class;
	rdfs:subClassOf prov:Activity;
	rdfs:label "ManufacturersCalibration"@en;
	rdfs:comment "The ManufacturersCalibration class describes instrument calibrations undertaken by their manufacturer.".

proc:InSituCorrection a rdfs:Class;
	rdfs:subClassOf prov:Activity;
	rdfs:label "InSituCorrection"@en;
	rdfs:comment "The InSituCorrection class describes offsets applied to sensor measurements determined after comparison with discrete measurements made on Sampling Specimens."@en.

proc:usedInstrument a rdf:Property;
	rdfs:label "usedInstrument"@en;
	rdfs:comment "Assigns an instrument to an Observation Process"@en;
	rdfs:subPropertyOf prov:wasAssociatedWith;
	rdfs:domain proc:ComplexProcess;
	rdfs:range proc:Instrument.

proc:StandardOperatingProcedure a rdfs:Class;
	rdfs:label "StandardOperatingProcedure"@en;
	rdfs:comment "The class StandardOperatingProcedure is used to contain a chain of ComplexProcesses which are commonly used together."@en.

om:Observation rdfs:subClassOf prov:Activity.

om:Process rdfs:subClassOf prov:Activity.

om:procedure rdfs:subPropertyOf prov:wasInformedBy;
	rdfs:domain om:Observation;
	rdfs:range om:Process.

sam:Specimen rdfs:subClassOf prov:Entity.

sam:Process rdfs:subClassOf prov:Activity.

sam:processingDetails rdfs:subPropertyOf prov:wasGeneratedBy;
	rdfs:domain sam:Specimen;
	rdfs:range sam:Process.
	
sam:Measure a rdfs:Class;
	rdfs:label "Measure"@en.

proc:partialMeasure a rdf:Property;
	rdfs:label "partialMeasure"@en;
	rdfs:domain sam:Measure;
	rdfs:range proc:PartialMeasure.
	
proc:PartialMeasure a rdfs:Class;
	rdfs:label "PartialMeasure"@en;
	rdfs:comment "The PartialMeasure class is for use where a sam:Specimen samples more than one matrix (such as air and water in pCO2 measurements."@en.

proc:matrix a rdf:Property;
	rdfs:label "matrix"@en;
	rdfs:comment "The property matrix links a PartialMeasure to a URL defining the environmental sphere of this PartialMeasure, e.g. atmosphere"@en;
	rdfs:domain proc:PartialMeasure.
	
proc:size a rdf:Property;
	rdfs:label "size"@en;
	rdfs:comment "The property size is define how much substance a PartialMeasure represents";
	rdfs:domain proc:PartialMeasure.
	
proc:uom a rdf:Property;
	rdfs:label "uom"@en;
	rdfs:comment "The property uom links an instance to a resource defining its units of measure"@en;
	rdfs:domain proc:PartialMeasure;
	rdfs:domain proc:Uncertainty;
	rdfs:domain proc:UnrangedLimitsOfDetection;
	rdfs:range rdfs:Resource.
	
cpm:ObservableProperty a rdfs:Class;
	rdfs:subClassOf skos:Concept;
	rdf:label "Observable Property"@en.
	
proc:uncertainty a rdf:Property;
	rdfs:subPropertyOf skos:related;
	rdfs:label "uncertainty"@en;
	rdfs:comment "Connects an instance of cpm:ObservableProperty to an instance of proc:Uncertainty"@en;
	rdfs:domain cpm:ObservableProperty;
	rdfs:range proc:Uncertainty.

proc:Uncertainty a rdfs:Class;
	rdfs:label "Uncertainty"@en;
	rdfs:comment "The Uncertainty class is used to give information about the accuracy, resolution, limits of detection etc... of the Result of an Observation associated with an Observable Property"@en;
	rdfs:subClassOf skos:Concept.
	
proc:term a rdf:Property;
	rdfs:label "term"@en;
	rdfs:comment "Links a proc:Uncertainty to an rdf:resource (such as a skos:Concept) describing the type of uncertainty recorded (e.g. Accuracy; Limit of Detection)"@en;
	rdfs:domain proc:Uncertainity;
	rdfs:range rdfs:Literal.

proc:finalStage a rdf:Property;
	rdfs:label "finalStage"@en;
	rdfs:comment "The property finalStage is used to connect a StandardOperatingProcedure to the last ComplexProcess used in the chain which makes up the StandardOperatingProcedure. A full chain can be created thus:"@en;
	rdfs:domain proc:StandardOperatingProcedure;
	rdfs:range proc:ComplexProcess.

proc:citation a rdf:Property;
	rdfs:label "citation"@en;
	rdfs:comment "The citation property is used to connect a ComplexProcess, Algorithm, InSituCorrection or StandardOperatingProcedure to a literature reference describing the process."@en;
	rdfs:domain proc:ComplexProcess;
	rdfs:domain proc:Algorithm;
	rdfs:domain proc:StandardOperatingProcedure;
	rdfs:domain proc:InSituCorrection;
	rdfs:range proc:Citation.
	
proc:responsibleOrganisation a rdf:Property;
	rdfs:label "responsibleOrganisation"@en;
	rdfs:comment "The responsibleOrganisation property connects an Algorithm, a ComplexProcess, an InSituCorrection, or a ManufacturersCalibration to the organisation responsible for that process, or part-process"@en;
	rdfs:domain proc:Algorithm;
	rdfs:domain proc:InSituCorrection;
	rdfs:domain proc:ComplexProcess;
	rdfs:domain proc:ManufacturersCalibration;
	rdfs:range rdfs:Resource.
	
proc:LimitsOfDetection a rdfs:Class;
	rdfs:label "LimitsOfDetection"@en;
	rdfs:comment "This is a super-class for describing accuracy, resolution, precision etc..."@en.

proc:RangedLimitsOfDetection a rdfs:Class;
	rdfs:label "RangedLimitsOfDetection"@en;
	rdfs:subClassOf proc:LimitsOfDetection.

proc:UnrangedLimitsOfDetection a rdfs:Class;
	rdfs:label "UnrangedLimitsOfDetection"@en;
	rdfs:subClassOf proc:LimitsOfDetection.

proc:value a rdfs:Property;
	rdfs:label "value"@en;
	rdfs:comment "The propety value links an Uncertainty or an UnrangedLimitOfDetection to the value associated with it."@en;
	rdfs:domain proc:UnrangedLimitsOfDetection;
	rdfs:domain proc:Uncertainty;
	rdfs:range rdfs:Literal.

proc:Accuracy a rdfs:Class;
	rdfs:subClassOf proc:UnrangedLimitsOfDetection;
	rdfs:label "Accuracy"@en.

proc:Precision a rdfs:Class;
	rdfs:subClassOf proc:UnrangedLimitsOfDetection;
	rdfs:label "Precision"@en.
	
proc:Resolution a rdfs:Class;
	rdfs:subClassOf proc:UnrangedLimitsOfDetection;
	rdfs:label "Resolution"@en.

proc:OperatingRange a rdfs:Class;
	rdfs:subClassOf proc:RangedLimitsOfDetection;
	rdfs:label "OperatingRange"@en.
	
proc:maximum a rdfs:Property;
	rdfs:label "maximum"@en;
	rdfs:domain proc:RangedLimitsOfDetection;
	rdfs:range proc:Maximum.
	
proc:minimum a rdfs:Property;
	rdfs:label "minimum"@en;
	rdfs:domain proc:RangedLimitsOfDetection;
	rdfs:range proc:Minimum.